src/PushButtonSynthesis/BaseConversion.v
@@ -102,7 +102,7 @@ Section __.
           {widen_carry : widen_carry_opt}
           {widen_bytes : widen_bytes_opt}
           {assembly_conventions : assembly_conventions_opt}
-          {errules : extra_rewrite_rules_opt}
+          {errules : extra_rewrite_rules}
           {error_on_unused_assembly_functions : error_on_unused_assembly_functions_opt}
           (s : Z) (c : list (Z * Z))
           (src_n : nat)
