src/PushButtonSynthesis/SaturatedSolinas.v
@@ -84,7 +84,7 @@ Section __.
           {widen_carry : widen_carry_opt}
           (widen_bytes : widen_bytes_opt := true) (* true, because we don't allow byte-sized things anyway, so we should not expect carries to be widened to byte-size when emitting C code *)
           {assembly_conventions : assembly_conventions_opt}
-          {errules : extra_rewrite_rules_opt}
+          {errules : extra_rewrite_rules}
           {error_on_unused_assembly_functions : error_on_unused_assembly_functions_opt}
           (s : Z)
           (c : list (Z * Z))
